add AST PTS frontier correspondence

theories/Eq/ProbabilisticPTS.v
@@ -3,9 +3,10 @@ Set Warnings "-ambiguous-paths".
 
 Require Import Utf8 Program.Equality.
 
+From Coinduction Require Import all.
 From PTree.Core Require Import PTreeDefinitionNew.
-From PTree.Prob Require Import FrontierLift.
-From PTree.Eq Require Import PWeakAbstract.
+From PTree.Prob Require Import FrontierLift MeasureIteration.
+From PTree.Eq Require Import PWeakAbstract PWeakUnbounded.
 
 Set Implicit Arguments.
 Unset Strict Implicit.
@@ -136,3 +137,207 @@ Proof.
 Qed.
 
 End FiniteCorrespondence.
+
+Section ASTWeakTransitions.
+Context {E : Type -> Type} {M : Type -> Type}
+  `{MI : MeasureInterface M}
+  `{MO : @MeasureOmegaInterface M MI}.
+
+(** AST weak transitions of the induced PTS.  Finite internal closure is
+    delegated to [ppts_weak]; unbounded loops are justified by the same
+    absorbing distribution iteration and total-mass condition used by the
+    measure semantics. *)
+Inductive ppts_ast_weak {R} :
+    ptree' E M R -> M (aphead E M R) -> Prop :=
+  | PPTSAFinite ot hs :
+      ppts_weak ot hs -> ppts_ast_weak ot hs
+  | PPTSATau t hs :
+      ppts_ast_weak (observe t) hs -> ppts_ast_weak (TauF t) hs
+  | PPTSAProb {X} (mu : M X) k
+      (front : X -> M (aphead E M R)) (Good : X -> Prop) :
+      meas_ae mu Good ->
+      (forall x, Good x -> ppts_ast_weak (observe (k x)) (front x)) ->
+      ppts_ast_weak (ProbF mu k) (meas_bind mu front)
+  | PPTSAIter {I}
+      (step : I -> ptree E M (I + R))
+      (transition : I -> M (I + R)) i out :
+      (forall j, ppts_weak (observe (step j))
+        (meas_bind (transition j)
+          (fun next => meas_ret (APHRet next)))) ->
+      meas_iter transition i out -> meas_total out ->
+      ppts_ast_weak (observe (PTree.iter step i))
+        (meas_bind out (fun r => meas_ret (APHRet r)))
+  | PPTSABind {A} (t : ptree E M A) (k : A -> ptree E M R)
+      hs (front : A -> M (aphead E M R)) :
+      ppts_ast_weak (observe t) hs ->
+      (forall a, ppts_ast_weak (observe (k a)) (front a)) ->
+      ppts_ast_weak (observe (PTree.bind t k))
+        (meas_bind hs (aphead_bind_front k front))
+  | PPTSANestedIter {I}
+      (step : I -> ptree E M (I + R))
+      (transition : I -> M (I + R)) i out :
+      (forall j, ppts_ast_weak (observe (step j))
+        (meas_bind (transition j)
+          (fun next => meas_ret (APHRet next)))) ->
+      meas_iter transition i out -> meas_total out ->
+      ppts_ast_weak (observe (PTree.iter step i))
+        (meas_bind out (fun r => meas_ret (APHRet r))).
+
+End ASTWeakTransitions.
+
+Section ASTCorrespondence.
+Context {E : Type -> Type} {M : Type -> Type}
+  `{MI : MeasureInterface M} `{MC : @MeasureCoreLaws M MI}
+  `{ML : @MeasureLaws M MI MC} `{MB : @MeasureBindLaws M MI}
+  `{MM : @MeasureMonadLaws M MI}
+  `{MG : @MeasureCongruenceLaws M MI}
+  `{MO : @MeasureOmegaInterface M MI}.
+
+Theorem aufrontier_to_ppts_ast_weak {R}
+    (ot : ptree' E M R) hs :
+  aufrontier ot hs -> ppts_ast_weak ot hs.
+Proof.
+  revert R ot hs. fix IH 4. intros R0 ot hs Hf. destruct Hf.
+  - exact (PPTSAFinite (apfrontier_to_ppts_weak H)).
+  - exact (PPTSATau (IH _ _ _ Hf)).
+  - apply PPTSAProb with (Good := Good); [exact H|].
+    intros x Hx. exact (IH _ _ _ (H0 x Hx)).
+  - eapply PPTSAIter; [|exact H0|exact H1].
+    intro j. exact (apfrontier_to_ppts_weak (H j)).
+  - apply PPTSABind.
+    + exact (IH _ _ _ Hf).
+    + intros a. match goal with
+      | Hk : forall x, aufrontier _ _ |- _ => exact (IH _ _ _ (Hk a))
+      end.
+  - apply PPTSANestedIter with (transition := transition).
+    + intros j. exact (IH _ _ _ (H j)).
+    + exact H0.
+    + exact H1.
+Qed.
+
+Theorem ppts_ast_weak_to_aufrontier {R}
+    (ot : ptree' E M R) hs :
+  ppts_ast_weak ot hs -> aufrontier ot hs.
+Proof.
+  revert R ot hs. fix IH 4. intros R0 ot hs Hw. destruct Hw.
+  - exact (AUFFinite (ppts_weak_to_apfrontier H)).
+  - exact (AUFTau (IH _ _ _ Hw)).
+  - apply AUFProb with (Good := Good); [exact H|].
+    intros x Hx. exact (IH _ _ _ (H0 x Hx)).
+  - eapply AUFIter; [|exact H0|exact H1].
+    intro j. exact (ppts_weak_to_apfrontier (H j)).
+  - apply AUFBind.
+    + exact (IH _ _ _ Hw).
+    + intros a. match goal with
+      | Hk : forall x, ppts_ast_weak _ _ |- _ => exact (IH _ _ _ (Hk a))
+      end.
+  - apply AUFNestedIter with (transition := transition).
+    + intros j. exact (IH _ _ _ (H j)).
+    + exact H0.
+    + exact H1.
+Qed.
+
+Theorem ppts_ast_weak_iff_aufrontier {R}
+    (ot : ptree' E M R) hs :
+  ppts_ast_weak ot hs <-> aufrontier ot hs.
+Proof.
+  split; [apply ppts_ast_weak_to_aufrontier|
+          apply aufrontier_to_ppts_ast_weak].
+Qed.
+
+End ASTCorrespondence.
+
+Section PTSBisimulation.
+Context {E : Type -> Type} {M : Type -> Type}
+  `{MI : MeasureInterface M} `{MC : @MeasureCoreLaws M MI}
+  `{MO : @MeasureOmegaInterface M MI}.
+Context {R1 R2 : Type}.
+Variable RR : R1 -> R2 -> Prop.
+
+(** Independent weak probabilistic bisimulation on the induced PTS: every
+    AST weak transition must be matchable by a coupled weak transition in
+    the other system. *)
+Definition ppts_bisimF
+    (sim : ptree E M R1 -> ptree E M R2 -> Prop)
+    (t1 : ptree E M R1) (t2 : ptree E M R2) : Prop :=
+  (forall hs1, ppts_ast_weak (observe t1) hs1 -> exists hs2,
+      ppts_ast_weak (observe t2) hs2 /\
+      meas_lift (aphead_rel RR sim) hs1 hs2) /\
+  (forall hs2, ppts_ast_weak (observe t2) hs2 -> exists hs1,
+      ppts_ast_weak (observe t1) hs1 /\
+      meas_lift (aphead_rel RR sim) hs1 hs2).
+
+Lemma ppts_bisimF_monotone sim1 sim2 :
+  (forall t1 t2, sim1 t1 t2 -> sim2 t1 t2) ->
+  forall t1 t2, ppts_bisimF sim1 t1 t2 -> ppts_bisimF sim2 t1 t2.
+Proof.
+  intros Hsim t1 t2 [HL HR]. split; intros hs Hweak.
+  - destruct (HL _ Hweak) as [hs' [Hw' Hlift]].
+    exists hs'. split; [exact Hw'|].
+    eapply meas_lift_mono; [|exact Hlift].
+    exact (aphead_rel_mono Hsim).
+  - destruct (HR _ Hweak) as [hs' [Hw' Hlift]].
+    exists hs'. split; [exact Hw'|].
+    eapply meas_lift_mono; [|exact Hlift].
+    exact (aphead_rel_mono Hsim).
+Qed.
+
+Program Definition fppts_bisim :
+    mon (ptree E M R1 -> ptree E M R2 -> Prop) :=
+  {| body := ppts_bisimF |}.
+Next Obligation.
+  intros sim1 sim2 Hsub t1 t2 H.
+  eapply ppts_bisimF_monotone; eauto.
+Qed.
+
+Definition ppts_bisim : ptree E M R1 -> ptree E M R2 -> Prop :=
+  gfp fppts_bisim.
+
+Lemma ppts_bisim_unfold t1 t2 :
+  ppts_bisim t1 t2 -> ppts_bisimF ppts_bisim t1 t2.
+Proof. intro H. apply (gfp_pfp fppts_bisim) in H. exact H. Qed.
+
+Lemma ppts_bisim_fold t1 t2 :
+  ppts_bisimF ppts_bisim t1 t2 -> ppts_bisim t1 t2.
+Proof. intro H. unfold ppts_bisim. apply (gfp_fp fppts_bisim). exact H. Qed.
+
+End PTSBisimulation.
+
+Section AuweakPTSSoundness.
+Context {E : Type -> Type} {M : Type -> Type}
+  `{MI : MeasureInterface M} `{MC : @MeasureCoreLaws M MI}
+  `{ML : @MeasureLaws M MI MC} `{MB : @MeasureBindLaws M MI}
+  `{MM : @MeasureMonadLaws M MI}
+  `{MG : @MeasureCongruenceLaws M MI}
+  `{MO : @MeasureOmegaInterface M MI}
+  `{UC : @UnboundedFrontierCoherence E M MI MO}.
+
+Theorem auweak_ppts_bisim_sound {R1 R2}
+    (RR : R1 -> R2 -> Prop) :
+  forall t1 t2,
+    @auweak E M MI MC MO R1 R2 RR t1 t2 ->
+    @ppts_bisim E M MI MC MO R1 R2 RR t1 t2.
+Proof.
+  unfold ppts_bisim. coinduction CH CIH.
+  intros t1 t2 Hrel. unfold fppts_bisim, ppts_bisimF; cbn.
+  assert (Hmatch : aufrontier_match RR (auweak RR)
+      (observe t1) (observe t2)).
+  { exact (auweakF_frontier_match (auweak_unfold Hrel)). }
+  destruct Hmatch as [HL HR]. split.
+  - intros hs1 Hpts1.
+    pose proof (ppts_ast_weak_to_aufrontier Hpts1) as Hf1.
+    destruct (HL _ Hf1) as [hs2 [Hf2 Hlift]].
+    exists hs2. split.
+    + exact (aufrontier_to_ppts_ast_weak Hf2).
+    + eapply meas_lift_mono; [|exact Hlift].
+      intros h1 h2 Hh. eapply aphead_rel_mono; [exact CIH|exact Hh].
+  - intros hs2 Hpts2.
+    pose proof (ppts_ast_weak_to_aufrontier Hpts2) as Hf2.
+    destruct (HR _ Hf2) as [hs1 [Hf1 Hlift]].
+    exists hs1. split.
+    + exact (aufrontier_to_ppts_ast_weak Hf1).
+    + eapply meas_lift_mono; [|exact Hlift].
+      intros h1 h2 Hh. eapply aphead_rel_mono; [exact CIH|exact Hh].
+Qed.
+
+End AuweakPTSSoundness.
